Env.v
@@ -1,0 +1,20 @@
+(* Environments that store their length as part of their type *)
+Require Import Coq.Vectors.Vector.
+Require Import Coq.Vectors.VectorDef.
+
+Notation "[]" := (nil _).
+Notation "h :: t" := (cons _ h _ t) (at level 60, right associativity).
+
+Definition env (A : Type) (n : nat) : Type :=
+  Vector.t (option A) n.
+
+Definition empty A n : env A n :=
+  const None n.
+
+(* Environment of length n with x = a. *)
+(* FIXME: finite integers? x < n *)
+Definition singleton A n x (a : A) : env A n :=
+  match x with
+  | O => Some a :: []
+  |
+  end.
